src/CPS/Conversion.v
@@ -1,26 +1,32 @@
 Require Import FunInd.
-From Src Require Import Tree.
-From CPS Require Import Tree.
+From Src Require Import Tree Fun_sem.
+From CPS Require Import Tree Fun_sem.
 From Common Require Import Literal Primitive.
+From Utils Require Import Env.
 
+Open Scope list_scope.
 
+Module ST := Src.Tree.
+Module SV := Src.Fun_sem.
+Module CT := CPS.Tree.
+Module CV := CPS.Fun_sem.
 
-Fixpoint cps_rec (nf: nat) (t: Src.Tree.term) (ctx: (nat * CPS.Tree.atom) -> (nat * CPS.Tree.term)): nat * CPS.Tree.term :=
+Fixpoint cps_rec (nf: nat) (t: ST.term) (ctx: (nat * CT.atom) -> (nat * CT.term)): nat * CT.term :=
   match t with 
-  | Src.Tree.Var n => ctx (nf, Var n)
-  | Src.Tree.Const l => ctx (nf, Lit l)
-  | Src.Tree.Let x t rest => 
+  | ST.Var n => ctx (nf, Var n)
+  | ST.Const l => ctx (nf, CT.Lit l)
+  | ST.Let x t rest => 
       let (nf', rest') := cps_rec nf rest ctx in
       cps_rec nf' t (fun r => 
         let (nf'', n) := r in
-        (nf'', CPS.Tree.LetU x Id n rest'))
-  | Src.Tree.LetRec (Src.Tree.Func fname farg fbody) rest =>
+        (nf'', CT.LetU x Id n rest'))
+  | ST.LetRec (ST.Fnt fname farg fbody) rest =>
       let retC := nf in
       let (nf', fbody') := cps_rec (nf + 1) fbody (fun r => 
-        let (nf_f, f) := r in (nf_f, CPS.Tree.AppC1 retC f)) in
+        let (nf_f, f) := r in (nf_f, CT.AppC1 retC f)) in
       let (nf'', rest') := cps_rec nf' rest ctx in 
-      (nf'', CPS.Tree.LetF (Fnt fname retC farg fbody') rest')
-  | Src.Tree.App f t =>
+      (nf'', CT.LetF (Fnt fname retC farg fbody') rest')
+  | ST.App f t =>
       let c := nf in
       let carg := nf + 1 in
       let (nf', cbody) := ctx (nf + 2, Var carg) in 
@@ -28,88 +34,117 @@ Fixpoint cps_rec (nf: nat) (t: Src.Tree.term) (ctx: (nat * CPS.Tree.atom) -> (na
         let (nf'', f') := r in
         cps_rec nf'' t (fun r' => 
           let (nf3, t') := r' in
-            (nf3, CPS.Tree.LetC (Cnt1 c carg cbody) (AppF f' c t'))
+            (nf3, CT.LetC (Cnt1 c carg cbody) (AppF f' c t'))
           )
         )
-  | Src.Tree.In => 
+  | ST.In => 
       let n := nf in
       let (nf', r) := ctx (nf + 1, Var n) in
-      (nf', CPS.Tree.LetIn n r)
-  | Src.Tree.Out t => 
+      (nf', CT.LetIn n r)
+  | ST.Out t => 
       let n := nf in
       let (nf', rest) := ctx (nf + 1, Var n) in
       cps_rec nf' t (fun r => 
         let (nf'', t') := r in 
-        (nf'', CPS.Tree.LetOut n t' rest)
+        (nf'', CT.LetOut n t' rest)
       )
-  | Src.Tree.Ite cond thent elset => 
+  | ST.Ite cond thent elset => 
       let c := nf in 
       let carg := nf + 1 in 
       let (nf', cbody) := ctx (nf + 2, Var carg) in 
       let thenc := nf' in 
       let (nf2, thent') := cps_rec (nf' + 1) thent (fun r => 
         let (nf3, t) := r in 
-        (nf3, CPS.Tree.AppC1 c t)
+        (nf3, CT.AppC1 c t)
       ) in 
       let elsec := nf2 in
       let (nf4, elset') := cps_rec (nf2 + 1) elset (fun r => 
         let (nf5, t) := r in 
-        (nf5, CPS.Tree.AppC1 c t)
+        (nf5, CT.AppC1 c t)
       ) in 
       cps_rec nf4 cond (fun r => 
         let (nf6, cond') := r in
-        (nf6, CPS.Tree.LetC (Cnt1 c carg cbody) (
-          CPS.Tree.LetC (Cnt0 thenc thent') (
-            CPS.Tree.LetC (Cnt0 elsec elset') (
-              CPS.Tree.Ite cond' thenc elsec
+        (nf6, CT.LetC (Cnt1 c carg cbody) (
+          CT.LetC (Cnt0 thenc thent') (
+            CT.LetC (Cnt0 elsec elset') (
+              CT.Ite cond' thenc elsec
             )
           )
         ))
       )
-  | Src.Tree.BinaryOp op t1 t2 => 
+  | ST.BinaryOp op t1 t2 => 
       let n := nf in
       cps_rec (nf + 1) t1 (fun r => 
         let (nf1, t1') := r in
         cps_rec nf1 t2 (fun r' =>
           let (nf2, t2') := r' in
           let (nf3, t) := ctx (nf2, Var n) in
-          (nf3, CPS.Tree.LetB n op t1' t2' t)
+          (nf3, CT.LetB n op t1' t2' t)
         )  
       )
-  | Src.Tree.UnaryOp op t =>
+  | ST.UnaryOp op t =>
       let n := nf in
       cps_rec (nf + 1) t (fun r => 
         let (nf1, t') := r in
         let (nf2, rest) := ctx (nf1, Var n) in
-        (nf2, CPS.Tree.LetU n op t' rest)
+        (nf2, CT.LetU n op t' rest)
       )
-  | Src.Tree.Match scrut (larg, lt) (rarg, rt) =>
+  | ST.Match scrut (larg, lt) (rarg, rt) =>
       let c := nf in 
       let carg := nf + 1 in 
       let (nf1, cbody) := ctx (nf + 2, Var carg) in 
-      let cnt := CPS.Tree.Cnt1 c carg cbody in
+      let cnt := CT.Cnt1 c carg cbody in
       let lc := nf1 in
       let (nf2, lbody) := cps_rec (nf1 + 1) lt (fun r => 
         let (nf3, lt') := r in
-        (nf3, CPS.Tree.AppC1 c lt')
+        (nf3, CT.AppC1 c lt')
       ) in
-      let lcnt := CPS.Tree.Cnt1 lc larg lbody in
+      let lcnt := CT.Cnt1 lc larg lbody in
       let rc := nf2 in
       let (nf4, rbody) := cps_rec (nf2 + 1) rt (fun r =>
         let (nf5, rt') := r in
-        (nf5, CPS.Tree.AppC1 c rt')
+        (nf5, CT.AppC1 c rt')
       ) in
-      let rcnt := CPS.Tree.Cnt1 rc rarg rbody in
+      let rcnt := CT.Cnt1 rc rarg rbody in
       cps_rec nf4 scrut (fun r => 
         let (nf6, scrut') := r in
-        (nf6, CPS.Tree.LetC cnt (
-          CPS.Tree.LetC lcnt (
-            CPS.Tree.LetC rcnt (
-              CPS.Tree.Match scrut' lc rc
+        (nf6, CT.LetC cnt (
+          CT.LetC lcnt (
+            CT.LetC rcnt (
+              CT.Match scrut' lc rc
             )
           )
         ))
       )
   end.
 
-
+Fixpoint cps_rec_v (nf : nat) (v : SV.value) {struct v} : nat * CV.value :=
+  match v with 
+  | SV.Lit l => (nf, CV.Lit l)
+  | SV.Tuple v1 v2 => 
+      let (nf1, v1') := cps_rec_v nf v1 in
+      let (nf2, v2') := cps_rec_v nf v2 in
+      (nf2, CV.Tuple v1' v2')
+  | SV.Left v => 
+      let (nf1, v') := cps_rec_v nf v in
+      (nf1, CV.Left v')
+  | SV.Right v => 
+      let (nf1, v') := cps_rec_v nf v in
+      (nf1, CV.Right v')
+  | SV.Fun (ST.Fnt fname farg fbody) env => 
+      let fix cps_rec_v_env nf env := 
+        match env with
+        | nil => (nf, nil)
+        | (n, v) :: env => 
+            let (nf', v') := cps_rec_v nf v in
+            let (nf'', env') := cps_rec_v_env nf' env in
+            (nf'', (n, v') :: env')
+        end in
+      let (nf', env') := cps_rec_v_env nf env in
+      let retC := nf' in
+      let (nf'', fbody') := cps_rec (nf' + 1) fbody (fun r =>
+        let (nf0, res) := r in
+        (nf0, CPS.Tree.AppC1 retC res)
+      ) in
+      (nf'', CV.Fun (CPS.Tree.Fnt fname retC farg fbody') env')
+  end.
