src/utils/Env.v
@@ -18,14 +18,22 @@ Fixpoint lookup {A: Type} (e : env A) (n: nat) : option A :=
 Definition add {A: Type} (e : env A) (n: nat) (a: A) : env A := 
   (n, a) :: e.
 
+Declare Scope env_scope.
+
+Notation "'{' '}'" := empty : env_scope.
+Notation "env '+' '(' k ',' v ')'" := (add env k v) 
+  (at level 50, left associativity) : env_scope.
+Notation "env '?' k" := (lookup env k) 
+  (at level 50, no associativity) : env_scope.
+
+Open Scope env_scope.
+
 Theorem lookup_empty: forall A k, lookup (@empty A) k = None.
-Proof.
-  auto.
-Qed.
+Proof. auto. Qed.
 
 Theorem lookup_add_eq: forall A (e : env A) n1 n2 v,
   n1 = n2 -> 
-    lookup (add e n1 v) n2 = Some v.
+    (e + (n1, v)) ? n2 = Some v.
 Proof.
   intros; simpl; subst.
   rewrite Nat.eqb_refl.
@@ -34,7 +42,7 @@ Qed.
 
 Theorem lookup_add_ne: forall A (e : env A) n1 n2 v,
   n1 <> n2 ->
-    lookup (add e n1 v) n2 = lookup e n2.
+    (e + (n1, v)) ? n2 = e ? n2.
 Proof.
   intros; simpl.
   apply_anywhere Nat.eqb_neq.
